dev/lf/mutation/tight/Substitution.v
@@ -250,16 +250,15 @@ Lemma subst_rules: forall y U,
     x \notin fv_env_types S1 ->
     ty_trm ty_general sub_general (G1 & (subst_env x y G2)) (S1 & subst_env x y S2) (trm_var (avar_f y)) (subst_typ x y U) ->
     ty_defs (G1 & (subst_env x y G2)) (S1 & subst_env x y S2) (subst_defs x y ds) (subst_typ x y T)) /\
-  (forall m1 m2 G S T V, subtyp m1 m2 G S T V -> forall G1 G2 S1 S2 x,
+  (forall m2 G S T V, subtyp m2 G S T V -> forall G1 G2 S1 S2 x,
     G = G1 & x ~ U & G2 ->
     ok (G1 & x ~ U & G2) ->
     x \notin fv_env_types G1 ->
     S = S1 & S2 ->
     x \notin fv_env_types S1 ->
     ty_trm ty_general sub_general (G1 & (subst_env x y G2)) (S1 & subst_env x y S2) (trm_var (avar_f y)) (subst_typ x y U) ->
-    m1 = ty_general ->
     m2 = sub_general ->
-    subtyp m1 m2 (G1 & (subst_env x y G2)) (S1 & subst_env x y S2) (subst_typ x y T) (subst_typ x y V)).
+    subtyp m2 (G1 & (subst_env x y G2)) (S1 & subst_env x y S2) (subst_typ x y T) (subst_typ x y V)).
 Proof.
   intros y S. apply rules_mutind; intros; subst.
   - (* ty_var *)
@@ -405,8 +404,8 @@ Proof.
   - (* subtyp_sel1 *)
     eapply subtyp_sel1.
     apply H; auto.
-  - (* subtyp_sel2_tight *) inversion H7.
-  - (* subtyp_sel1_tight *) inversion H7.
+  - (* subtyp_sel2_tight *) inversion H6.
+  - (* subtyp_sel1_tight *) inversion H6.
   - (* subtyp_all *)
     simpl. apply_fresh subtyp_all as z; auto.
     assert (z \notin L) as FrL by auto.
