dev/lf/tight-proof/General_to_tight.v
@@ -17,8 +17,8 @@ Lemma tight_to_precise_typ_dec: forall G x A S U,
   ty_trm ty_general sub_tight G (trm_var (avar_f x)) (typ_rcd (dec_typ A S U)) ->
   exists T,
     ty_trm ty_precise sub_general G (trm_var (avar_f x)) (typ_rcd (dec_typ A T T)) /\
-    subtyp ty_general sub_tight G T U /\
-    subtyp ty_general sub_tight G S T.
+    subtyp sub_tight G T U /\
+    subtyp sub_tight G S T.
 Proof.
   introv HG Ht.
   lets Htp: (tight_possible_types_lemma HG Ht). clear Ht.
@@ -35,7 +35,7 @@ Lemma tight_to_precise_trm_dec: forall G x a T,
   ty_trm ty_general sub_tight G (trm_var (avar_f x)) (typ_rcd (dec_trm a T)) ->
   exists T',
     ty_trm ty_precise sub_general G (trm_var (avar_f x)) (typ_rcd (dec_trm a T')) /\
-    subtyp ty_general sub_tight G T' T.
+    subtyp sub_tight G T' T.
 Proof.
   introv Hgd Ht.
   lets Htp: (tight_possible_types_lemma Hgd Ht). clear Ht.
@@ -51,10 +51,10 @@ Lemma tight_to_precise_typ_all: forall G x S T,
   ty_trm ty_general sub_tight G (trm_var (avar_f x)) (typ_all S T) ->
   exists S' T' L,
     ty_trm ty_precise sub_general G (trm_var (avar_f x)) (typ_all S' T') /\
-    subtyp ty_general sub_tight G S S' /\
+    subtyp sub_tight G S S' /\
     (forall y,
         y \notin L ->
-            subtyp ty_general sub_general (G & y ~ S) (open_typ y T') (open_typ y T))
+            subtyp sub_general (G & y ~ S) (open_typ y T') (open_typ y T))
     .
 Proof.
   introv HG Ht.
@@ -65,14 +65,14 @@ Proof.
     destruct IHHtp as [S' [T' [L' [Hpt [HSsub HTsub]]]]].
     exists S' T' (dom G \u L \u L').
     split; auto.
-    assert (Hsub2 : subtyp ty_general sub_tight G (typ_all S0 T0) (typ_all S T)).
+    assert (Hsub2 : subtyp sub_tight G (typ_all S0 T0) (typ_all S T)).
     { apply subtyp_all with (L:=L); assumption. }
     split.
     + eapply subtyp_trans; eauto.
     + intros y Fr.
       assert (Hok: ok (G & y ~ S)) by auto using ok_push, inert_ok.
       apply tight_to_general in H; auto.
-      assert (Hnarrow: subtyp ty_general sub_general (G & y ~ S) (open_typ y T') (open_typ y T0)).
+      assert (Hnarrow: subtyp sub_general (G & y ~ S) (open_typ y T') (open_typ y T0)).
       { eapply narrow_subtyping; auto using subenv_last. }
       eauto.
 Qed.
@@ -81,8 +81,8 @@ Qed.
 Lemma tight_subtyping_sel: forall G x A S U,
     inert G ->
     ty_trm ty_general sub_tight G (trm_var (avar_f x)) (typ_rcd (dec_typ A S U)) ->
-    (subtyp ty_general sub_tight G (typ_sel (avar_f x) A) U /\
-     subtyp ty_general sub_tight G S (typ_sel (avar_f x) A)).
+    (subtyp sub_tight G (typ_sel (avar_f x) A) U /\
+     subtyp sub_tight G S (typ_sel (avar_f x) A)).
 Proof.
   introv HG Hty.
   pose proof (tight_to_precise_typ_dec HG Hty) as [T [Ht [Hs1 Hs2]]].
@@ -100,12 +100,11 @@ Lemma general_to_tight: forall G0,
      m1 = ty_general ->
      m2 = sub_general ->
      ty_trm ty_general sub_tight G t T) /\
-  (forall m1 m2 G S U,
-     subtyp m1 m2 G S U ->
+  (forall m2 G S U,
+     subtyp m2 G S U ->
      G = G0 ->
-     m1 = ty_general ->
      m2 = sub_general ->
-     subtyp ty_general sub_tight G S U).
+     subtyp sub_tight G S U).
 Proof.
   intros G0 HG.
   apply ts_mutind; intros; subst; try solve [eapply tight_subtyping_sel; auto]; eauto.
