dev/lf/tight-proof/Tight_possible_types_val.v
@@ -29,9 +29,9 @@ Inductive tight_pt_v : ctx -> val -> typ -> Prop :=
   (* Forall *)
 | t_pt_all_v : forall L G v S T S' T',
   tight_pt_v G v (typ_all S T) ->
-  subtyp ty_general sub_tight G S' S ->
+  subtyp sub_tight G S' S ->
   (forall y, y \notin L ->
-   subtyp ty_general sub_general (G & y ~ S') (open_typ y T) (open_typ y T')) ->
+   subtyp sub_general (G & y ~ S') (open_typ y T) (open_typ y T')) ->
   tight_pt_v G v (typ_all S' T')
   (* Tight Selection *)
 | t_pt_sel_v : forall G v y A S,
@@ -52,7 +52,7 @@ Hint Constructors tight_pt_v.
 Lemma tight_possible_types_closure_tight_v: forall G v T U,
   inert G ->
   tight_pt_v G v T ->
-  subtyp ty_general sub_tight G T U ->
+  subtyp sub_tight G T U ->
   tight_pt_v G v U.
 Proof.
   introv Hgd HT Hsub.
